removed log assumption

theories/prob_eff_lang/probblaze/examples/DH_KE/sec_channel_prf.v
@@ -37,9 +37,15 @@ Section schan_security.
   Hypothesis Bij_xor_sem : ∀ g1 g2 : vgG, group_xor_sem (group_xor_sem g1 g2) g2 = g1.
   Hypothesis Bij_xor_sem_l : ∀ g1 g2 : vgG, group_xor_sem g1 (group_xor_sem g1 g2) = g2.
   Hypothesis vg_int_xor_sem : ∀ g1 g2 : vgG, vg_of_int_sem (xor_sem (int_of_vg_sem g1) (int_of_vg_sem g2)) = Some (group_xor_sem g1 g2 ).
-  Variable log__g : vgG -> fin (S (S n'')).
-  Hypothesis Val_log : ∀ x : vgG, (g ^+(log__g x))%g = x.
-  Hypothesis Bij_log : forall m : vgG, @Bij (fin (S (S n''))) (fin (S (S n''))) (λ n, log__g (group_xor_sem m (g ^+n))).
+  Definition log__g : vgG -> fin (S (S n'')) := fun xg => match log_g xg with 
+                                                        | exist k _ => k 
+                                                        end.
+  Lemma val_log : ∀ x : vgG, (g ^+ (log__g x))%g = x.
+  Proof. 
+    intros. unfold log__g.
+    by destruct (log_g x) as [k Hk]. 
+  Qed. 
+    Hypothesis Bij_log : forall m : vgG, @Bij (fin (S (S n''))) (fin (S (S n''))) (λ n, log__g (group_xor_sem m (g ^+n))).
 
   Definition atokN' : namespace := nroot .@ "atokN1".
   Definition btokN' : namespace := nroot .@ "btokN1".
@@ -426,7 +432,7 @@ Lemma F_OAUTH_CHAN_SIM (f1 f2 : val) (L : sem_row Σ) :
                                        ∀ (leakauth1 leakauth2 keyleak1 keyleak2 : label),
                                        BREL v1 ((λ: "m", do: leakauth1 (Send "m")), (λ: "m", do: leakauth1 (Recv "m")))%V ((λ: "m", do: keyleak1 (Send "m")), (λ: "m", do: keyleak1 (Recv "m")))%V ≤ v2 ((λ: "m", do: leakauth2 (Send "m")), (λ: "m", do: leakauth2 (Recv "m")))%V ((λ: "m", do: keyleak2 (Send "m")), (λ: "m", do: keyleak2 (Recv "m")))%V  <| (iLblSig_to_iLblThy (envsec_row keyleak1 keyleak2 leakauth1 leakauth2 )) ++ (iLblSig_to_iLblThy L) |> {{ (λ w1 w2, 𝟙%T w1 w2)}}}}.
 Proof with (repeat foldkont) using  Bij_log Bij_xor_sem Bij_xor_sem_l G
-H Val_log XOR_spec0 cg group_xor_sem inG0
+H XOR_spec0 cg group_xor_sem inG0
 inG1 inG2 klk1 klk2 lka1 lka2 log__g vg
 vg_int_xor_sem vgg xor_struct Σ.
   iIntros "Hrelf1f2".
@@ -1215,8 +1221,7 @@ Lemma SEM_R_CHAN_SIM (f1 f2 : val) (L : sem_row Σ) :
     BREL R_CHAN f1
       ≤ CHAN_SIM_lazy (F_CHAN f2) <|⊥|> {{λ v1 v2,
                                        (∀ᵣ θ₁, ∀ᵣ θ₂,  (((𝔾 × (𝟙 + 𝟙)) -{ θ₁ }-> 𝟙) × ((𝟙 + 𝟙) -{ θ₁ }-> Option 𝟙)) ⊸ (((𝟙 + 𝟙) -{ θ₂ }-> 𝟙) ×(𝟙 + 𝟙) -{ θ₂ }-> Option 𝟙) -{ sem_row_union θ₁ (sem_row_union θ₂ L) }-∘ 𝟙)%T v1 v2 }}. 
-Proof with (repeat foldkont) using   Bij_log Bij_xor_sem Bij_xor_sem_l G H
-Val_log XOR_spec0 cg group_xor_sem log__g vg
+Proof with (repeat foldkont) using   Bij_log Bij_xor_sem Bij_xor_sem_l G H XOR_spec0 cg group_xor_sem log__g vg
 vg_int_xor_sem vgg xor_struct Σ.
 
  iIntros "Hrelf1f2".
@@ -1712,7 +1717,7 @@ vg_int_xor_sem vgg xor_struct Σ.
                                unfold g_sem. simpl. unfold sem_ty_prod.
                                iExists (vgval (group_xor_sem m (valgroup.g ^+ c))) , (vgval (valgroup.g ^+ f m c)) , bob , bob.
                                repeat (iSplit); try (iPureIntro); try reflexivity.
-                               + auto. simpl. unfold f. rewrite -> Val_log. exists (group_xor_sem m (g ^+ c)).
+                               + auto. simpl. unfold f. rewrite -> val_log. exists (group_xor_sem m (g ^+ c)).
                                  repeat split; reflexivity.
                                + simpl. exists #()%V, #()%V. repeat split; unfold bob; try reflexivity.
                                  left. repeat split; reflexivity. }
@@ -2084,8 +2089,7 @@ Lemma SEM_R_CHAN_SIM_rev (f1 f2 : val) (L : sem_row Σ) :
     BREL CHAN_SIM_lazy (F_CHAN f1)
       ≤ (R_CHAN f2) <|⊥|> {{λ v1 v2,
                               (∀ᵣ θ₁, ∀ᵣ θ₂,  (((𝔾 × (𝟙 + 𝟙)) -{ θ₁ }-> 𝟙) × ((𝟙 + 𝟙) -{ θ₁ }-> Option 𝟙)) ⊸ (((𝟙 + 𝟙) -{ θ₂ }-> 𝟙) ×(𝟙 + 𝟙) -{ θ₂ }-> Option 𝟙) -{ sem_row_union θ₁ (sem_row_union θ₂ L) }-∘ 𝟙)%T v1 v2 }}.
-Proof with (repeat foldkont) using   Bij_log Bij_xor_sem Bij_xor_sem_l G H
-Val_log XOR_spec0 cg group_xor_sem log__g vg
+Proof with (repeat foldkont) using   Bij_log Bij_xor_sem Bij_xor_sem_l G H XOR_spec0 cg group_xor_sem log__g vg
 vg_int_xor_sem vgg xor_struct Σ.
 
  iIntros "Hrelf1f2".  
@@ -2656,7 +2660,7 @@ split.
                                iExists (vgval (valgroup.g ^+ c)) , (vgval (group_xor_sem m (valgroup.g ^+ f m c))) , bob , bob.
                                repeat (iSplit); try (iPureIntro); try reflexivity.
                                + auto. simpl. unfold f. case_decide as Hc'; [| exfalso; lia].
-                                 rewrite -> Val_log.
+                                 rewrite -> val_log.
                                  rewrite -> Bij_xor_sem_l.
                                  assert (fin_to_nat (nat_to_fin Hc') = c)
                                  as -> by apply fin_to_nat_to_fin.
@@ -3031,8 +3035,7 @@ Lemma R_CHAN_CHAN_SIM_F_CHAN :
   ⊢ sem_val_typed (R_CHAN)%V (λ: "f", CHAN_SIM_lazy (F_CHAN "f"))%V
       (∀ᵣ θ__L ,(∀ᵣ θₕ, (((sem_ty_nat -{ θₕ }->  𝟙) × (𝟙 -{ θₕ }-> (Option  𝔾))) -{ sem_row_union  θₕ θ__L }-∘ 𝟙)) ⊸ (*type of client*)
       (∀ᵣ θ₁, ∀ᵣ θ₂,  (((𝔾 × (𝟙 + 𝟙)) -{ θ₁ }-> 𝟙) × ((𝟙 + 𝟙) -{ θ₁ }-> Option 𝟙)) ⊸ (((𝟙 + 𝟙) -{ θ₂ }-> 𝟙) × (𝟙 + 𝟙) -{ θ₂ }-> Option 𝟙) -{ sem_row_union θ₁ (sem_row_union θ₂ θ__L) }-∘ 𝟙))%T.
-Proof using  Bij_log Bij_xor_sem Bij_xor_sem_l G H
-Val_log XOR_spec0 cg group_xor_sem inG0 inG1 inG2
+Proof using  Bij_log Bij_xor_sem Bij_xor_sem_l G H XOR_spec0 cg group_xor_sem inG0 inG1 inG2
 log__g vg vg_int_xor_sem vgg xor_struct Σ.
   iModIntro. iIntros (L).
   iIntros (f1 f2) "Hrelf1f2".
@@ -3051,7 +3054,7 @@ Lemma CHAN_SIM_F_CHAN_R_CHAN :
       (∀ᵣ θ__L ,(∀ᵣ θₕ, (((sem_ty_nat -{ θₕ }->  𝟙) × (𝟙 -{ θₕ }-> (Option  𝔾))) -{ sem_row_union  θₕ θ__L }-∘ 𝟙)) ⊸ (*type of client*)
                 (∀ᵣ θ₁, ∀ᵣ θ₂,  (((𝔾 × (𝟙 + 𝟙)) -{ θ₁ }-> 𝟙) × ((𝟙 + 𝟙) -{ θ₁ }-> Option 𝟙)) ⊸ (((𝟙 + 𝟙) -{ θ₂ }-> 𝟙) × (𝟙 + 𝟙) -{ θ₂ }-> Option 𝟙) -{ sem_row_union θ₁ (sem_row_union θ₂ θ__L) }-∘ 𝟙))%T.
  Proof using  Bij_log Bij_xor_sem
-Bij_xor_sem_l G H Val_log XOR_spec0 cg
+Bij_xor_sem_l G H XOR_spec0 cg
 group_xor_sem inG0 inG1 inG2 log__g vg
 vg_int_xor_sem vgg xor_struct Σ.
   iModIntro. iIntros (L).
@@ -3072,8 +3075,7 @@ Lemma R_I_SCHAN :
   ⊢ sem_typed [] R_CHAN (λ: "f", (CHAN_SIM_lazy (F_CHAN "f")))%V ⊥
        (∀ᵣ θ__L ,(∀ᵣ θₕ, (((sem_ty_nat -{ θₕ }-> 𝟙) × (𝟙 -{ θₕ }-> (Option  𝔾))) -{ sem_row_union  θₕ θ__L }-∘ 𝟙)) ⊸ (*type of client*)
                  (∀ᵣ θ₁, ∀ᵣ θ₂,  (((𝔾 × (𝟙 + 𝟙)) -{ θ₁ }-> 𝟙) × ((𝟙 + 𝟙) -{ θ₁ }-> Option 𝟙)) ⊸ (((𝟙 + 𝟙) -{ θ₂ }-> 𝟙) × ((𝟙 + 𝟙) -{ θ₂ }-> Option 𝟙)) -{ sem_row_union θ₁ (sem_row_union θ₂ θ__L) }-∘ 𝟙))%T [].
-Proof using  Bij_log Bij_xor_sem Bij_xor_sem_l G H
-Val_log XOR_spec0 cg group_xor_sem inG0 inG1 inG2
+Proof using  Bij_log Bij_xor_sem Bij_xor_sem_l G H XOR_spec0 cg group_xor_sem inG0 inG1 inG2
 klk1 klk2 lka1 lka2 log__g vg vg_int_xor_sem vgg
 xor_struct Σ.
   iIntros (vs) "!# H". simpl.
@@ -3091,7 +3093,7 @@ Lemma I_R_SCHAN :
        (∀ᵣ θ__L ,(∀ᵣ θₕ, (((sem_ty_nat -{ θₕ }-> 𝟙) × (𝟙 -{ θₕ }-> (Option  𝔾))) -{ sem_row_union  θₕ θ__L }-∘ 𝟙)) ⊸ (*type of client*)
                  (∀ᵣ θ₁, ∀ᵣ θ₂,  (((𝔾 × (𝟙 + 𝟙)) -{ θ₁ }-> 𝟙) × ((𝟙 + 𝟙) -{ θ₁ }-> Option 𝟙)) ⊸ (((𝟙 + 𝟙) -{ θ₂ }-> 𝟙) × ((𝟙 + 𝟙) -{ θ₂ }-> Option 𝟙)) -{ sem_row_union θ₁ (sem_row_union θ₂ θ__L) }-∘ 𝟙))%T [].
 Proof using Bij_log Bij_xor_sem
-Bij_xor_sem_l G H Val_log XOR_spec0 cg
+Bij_xor_sem_l G H XOR_spec0 cg
 group_xor_sem inG0 inG1 inG2 klk1 klk2 lka1 lka2
 log__g vg vg_int_xor_sem vgg xor_struct Σ. 
   iIntros (vs) "!# H". simpl.
